Fixed some major issues with the LustreAst to Lustre conversion

compiler/parser.mly
@@ -28,7 +28,7 @@
 %left EQ
 %left ELSE
 
-%start<string * (binder list) *(binder list) * binder * ((int*exp) list)> node
+%start<string * ((binder*coq_type) list) * ((binder*coq_type) list) * (binder*coq_type) * ((int*exp) list)> node
 
 %%
 
@@ -54,7 +54,7 @@ node:
     LET
       eqs = equation_list
     TEL EOF
-    { (name, args,[], ret, eqs) }
+    { (name, args, [], ret, eqs) }
 
 returns:
   | RETURN ret = ident COLON typ=typ {(ret,typ)}
@@ -92,21 +92,21 @@ const:
 
 expr:
   | LPAREN e = expr RPAREN    { e }
-  | c = const                 { EConst(c) }
-  | v = var                   { EVar((v, TBool)) }
-  | e1 = expr AND e2 = expr   { EBinop(Bop_and, e1, e2) }
-  | e1 = expr OR e2 = expr    { EBinop(Bop_or, e1, e2) }
-  | e1 = expr XOR e2 = expr   { EBinop(Bop_xor, e1, e2) }
-  | e1 = expr PLUS e2 = expr  { EBinop(Bop_plus, e1, e2) }
-  | e1 = expr MINUS e2 = expr { EBinop(Bop_minus, e1, e2) }
-  | e1 = expr TIMES e2 = expr { EBinop(Bop_mult, e1, e2) }
-  | e1 = expr DIV e2 = expr   { EBinop(Bop_div, e1, e2) }
-  | e1 = expr GE e2 = expr    { EBinop(Bop_ge, e1, e2) }
-  | e1 = expr LE e2 = expr    { EBinop(Bop_le, e1, e2) }
-  | e1 = expr GT e2 = expr    { EBinop(Bop_gt, e1, e2) }
-  | e1 = expr LT e2 = expr    { EBinop(Bop_lt, e1, e2) }
-  | e1 = expr EQ e2 = expr    { EBinop(Bop_eq, e1, e2) }
-  | NOT e1 = expr             {EUnop(Uop_not,e1)}
-  | MINUS e1 = expr           {EUnop(Uop_neg,e1)}
-  | IF cond=expr THEN e1=expr ELSE e2=expr {EIfte(cond,e1,e2)}
+  | c = const                 { EConst c }
+  | v = var                   { EVar v }
+  | e1 = expr AND e2 = expr   { EBinop (Bop_and, e1, e2) }
+  | e1 = expr OR e2 = expr    { EBinop (Bop_or, e1, e2) }
+  | e1 = expr XOR e2 = expr   { EBinop (Bop_xor, e1, e2) }
+  | e1 = expr PLUS e2 = expr  { EBinop (Bop_plus, e1, e2) }
+  | e1 = expr MINUS e2 = expr { EBinop (Bop_minus, e1, e2) }
+  | e1 = expr TIMES e2 = expr { EBinop (Bop_mult, e1, e2) }
+  | e1 = expr DIV e2 = expr   { EBinop (Bop_div, e1, e2) }
+  | e1 = expr GE e2 = expr    { EBinop (Bop_ge, e1, e2) }
+  | e1 = expr LE e2 = expr    { EBinop (Bop_le, e1, e2) }
+  | e1 = expr GT e2 = expr    { EBinop (Bop_gt, e1, e2) }
+  | e1 = expr LT e2 = expr    { EBinop (Bop_lt, e1, e2) }
+  | e1 = expr EQ e2 = expr    { EBinop (Bop_eq, e1, e2) }
+  | NOT e1 = expr             { EUnop (Uop_not, e1) }
+  | MINUS e1 = expr           { EUnop (Uop_neg, e1) }
+  | IF cond=expr THEN e1=expr ELSE e2=expr { EIfte (cond,e1,e2) }
 ;
